SecureMessaging.lean
@@ -45,6 +45,8 @@ import SecureMessaging.PRFPRNG.Defs
 import SecureMessaging.PRP.Defs
 import SecureMessaging.SCKA.Defs
 import SecureMessaging.SCKA.MLKEMBraid.Authenticator
+import SecureMessaging.SCKA.MLKEMBraid.Basic
+import SecureMessaging.SCKA.MLKEMBraid.Construction
 import SecureMessaging.SCKA.SPQR.Unchunked
 import SecureMessaging.SCKA.OppUniKEM.Construction
 import SecureMessaging.SCKA.OppUniKEM.Correctness
